IT WORKS!

src/data.lean
@@ -1,6 +1,7 @@
 
 import .table .rule .rule_table
 namespace robot
+open tactic
 section equiv
     universes u
     variables {α : Type u} [has_lt α]
@@ -12,30 +13,40 @@ meta inductive task : Type
 |CreateAll : expr → task
 |Create : expr → task
 open task
-meta def task.code : task → ℕ
-|(task.Create _) := 0
-|(task.CreateAll _) := 1
-meta def task.lt : task → task → bool
-|(task.Create e₁) (task.Create e₂) := e₁ < e₂
-|(task.CreateAll e₁) (task.CreateAll e₂) := e₁ < e₂
-|x y := task.code x < task.code y
-meta instance task.has_lt : has_lt task := ⟨λ x y, task.lt x y⟩
-meta instance task.decidable_lt: decidable_rel ((<) : task → task → Prop) := by apply_instance
-
+namespace task
+    meta def code : task → ℕ
+    |(Create _) := 0
+    |(CreateAll _) := 1
+    meta def lt : task → task → bool
+    |(Create e₁) (Create e₂) := e₁ < e₂
+    |(CreateAll e₁) (CreateAll e₂) := e₁ < e₂
+    |x y := code x < code y
+    meta instance has_lt : has_lt task := ⟨λ x y, lt x y⟩
+    meta instance decidable_lt : decidable_rel ((<) : task → task → Prop) := by apply_instance
+    meta instance : has_to_tactic_format task := ⟨λ t, match t with
+    |(Create x) := pure (λ x, "Create " ++ x) <*> tactic.pp x
+    |(CreateAll x) := pure (λ x, "CreateAll " ++ x) <*> tactic.pp x
+    end⟩
+end task
 meta inductive strategy : Type
 |Use : rule → strategy
 |ReduceDistance : expr → expr → strategy
 open strategy
-meta def strategy.code : strategy → ℕ
-|(Use _) := 0
-|(ReduceDistance _ _) := 1
-meta def strategy.lt : strategy → strategy → bool
-|(Use r₁) (Use r₂) := r₁ < r₂
-|(ReduceDistance a b) (ReduceDistance a' b') := (a,b) < (a',b')
-|s₁ s₂ := s₁.code < s₂.code
-meta instance strategy.has_lt : has_lt strategy := ⟨λ x y, strategy.lt x y⟩
-meta instance strategy.decidable_lt : decidable_rel ((<) : strategy → strategy → Prop) := by apply_instance
-
+namespace strategy
+    meta def code : strategy → ℕ
+    |(Use _) := 0
+    |(ReduceDistance _ _) := 1
+    meta def lt : strategy → strategy → bool
+    |(Use r₁) (Use r₂) := r₁ < r₂
+    |(ReduceDistance a b) (ReduceDistance a' b') := (a,b) < (a',b')
+    |s₁ s₂ := s₁.code < s₂.code
+    meta instance has_lt : has_lt strategy := ⟨λ x y, lt x y⟩
+    meta instance decidable_lt : decidable_rel ((<) : strategy → strategy → Prop) := by apply_instance
+    meta instance : has_to_tactic_format robot.strategy := ⟨λ s, match s with
+        | (Use x) := do x ← tactic.pp x, pure $ "Use " ++ x
+        | (ReduceDistance x y) := pure (λ x y, "ReduceDistance " ++ x ++ " " ++ y) <*> tactic.pp x <*> tactic.pp y
+     end⟩
+end strategy
 -- meta inductive V
 -- |Task : task → V
 -- |Strategy : strategy → V
@@ -61,8 +72,6 @@ meta instance strategy.decidable_lt : decidable_rel ((<) : strategy → strategy
 -- meta def G := digraph V E
 -- meta instance : has_mem V G := digraph.has_mem
 
-meta structure config := 
-(rule_table     : rule_table)
 -- meta structure state :=
 -- (ce             : expr)
 -- (lookahead      : list rule)
@@ -72,19 +81,27 @@ meta structure config :=
 -- (acheived_tasks : table task)       -- a set of tasks that have recently been achieved and which should not be unachieved until their parent is achieved.
 -- (config         : config)           -- some data that should remain fixed for the duration of the tactic. [NOTE] maybe put in a reader monad?
 
+
 meta inductive stack_entry : Type
 |strategy (current : strategy)  : stack_entry
 |task  (current : task) (siblings : list task) (achieved : list task) : stack_entry
-meta instance stack_entry.of_strat : has_coe (strategy) (stack_entry) := ⟨stack_entry.strategy⟩
+namespace stack_entry
+    meta instance of_strat : has_coe (robot.strategy) (stack_entry) := ⟨stack_entry.strategy⟩
+    meta instance has_to_tactic_format : has_to_tactic_format (stack_entry) := ⟨λ s, match s with
+    |(strategy s) := tactic.pp s
+    |(task c s a) := tactic.pp c
+    end
+    ⟩
+end stack_entry
 meta def stack := list stack_entry
+namespace stack
+    meta instance : has_to_tactic_format stack := ⟨λ s : list stack_entry, tactic.pp s⟩
+end stack
 meta structure state :=
 (lookahead : list rule)
 (visited : table expr)
 -- (stack : stack)
-(config : config)
-
-
--- [TODO] proof object.
+(rt : rule_table)
 
 /-- The robot monad. -/
 meta def M : Type → Type := state_t state conv
@@ -94,8 +111,13 @@ meta instance : alternative M := state_t.alternative
 meta instance of_tactic {α} : has_coe (tactic α) (M α) := ⟨state_t.lift⟩
 meta instance of_conv {α} : has_coe (conv α) (M α) := ⟨state_t.lift⟩
 meta def map_state  (f : state → state) : M unit := (f <$> get) >>= put
-meta def get_rule_table : M rule_table := config.rule_table <$> state.config <$> get
-meta def get_ce : M expr := state_t.lift conv.lhs
+meta def get_rule_table : M rule_table := state.rt <$> get
+meta def add_rule : rule → M unit := λ r, do
+    s ← get,
+    rt ← s.rt.insert r,
+    put $ { rt := rt, ..s}
+
+meta def get_ce : M expr := state_t.lift (conv.lhs >>= instantiate_mvars)
 meta def get_visited : M $ table $ expr := state.visited <$> get
 meta def get_lookahead : M (list rule) := state.lookahead <$> get
 meta def M.hypothetically {α} : M α → M (option α) := λ tac, ⟨λ s, do
@@ -114,9 +136,18 @@ meta def stack.mfold_achieved {T} [monad T] {α} (f : α → task → T α) : α
 
 meta def refinement := list task × list strategy
 
-meta def task.test : task → M bool
-|(task.Create e) := do ce ← get_ce, pure $ expr.occurs e ce
-|_ := notimpl
+meta def task.test : expr → task → M bool
+|ce (task.Create e) := do
+    e ← instantiate_mvars e,
+    pp_ce ← pp ce, pp_e ← pp e,
+    --trace_m "task.test: " $ (to_fmt "testing that " ++ pp_ce ++ " satisfies Create " ++ pp_e),
+    matches : list ez.zipper ← ez.zipper.find_occurences ce e ,
+    --trace_m "task.test: " $ matches,
+    pure $ bnot matches.empty
+|ce t@(task.CreateAll e) := do
+    trace_m "task.test: " $ t,
+    o ← hypothetically (unify e ce), 
+    pure o.is_some
 meta def strategy.of_rule : rule → M strategy := λ r, pure $ strategy.Use $ r
 
 /-- Do In One Move. Check the lookahead table and see if any of the entries in there cause the task to be achieved. -/
@@ -127,9 +158,12 @@ meta def task.diom : task → M (list strategy) := λ t, do
         let rhs := rule.rhs r,
         let pf := rule.pf r,
         x : option rule ← M.hypothetically (do
-                conv.update_lhs rhs pf, 
-                result ← task.test t, 
-                if result then pure r else tactic.fail ""
+                result ← task.test rhs t,
+                if result then do
+                    ppr ← pp r, 
+                    trace_m "task.diom: " $ (to_fmt "found a rule: ") ++ ppr,
+                    pure r,
+                pure r else tactic.fail ""
         ),
         match x with
         |(some r) := pure r
@@ -139,7 +173,11 @@ meta def task.diom : task → M (list strategy) := λ t, do
     winners.mmap (strategy.of_rule)
 open ez
 
-meta def try_dioms : task → M refinement | t := do dioms ← task.diom t, if ¬ dioms.empty then pure ([],dioms) else failure
+meta def try_dioms : task → M refinement | t := do 
+    -- trace "trying dioms",
+    dioms ← task.diom t, 
+    --trace dioms,
+    if ¬ dioms.empty then pure ([],dioms) else failure
 
 meta def task.refine (t : task) : M refinement :=
 try_dioms t <|>
@@ -152,6 +190,7 @@ match t with
     pure $ ([],strats)
 |(task.CreateAll a) := do
     ce ← get_ce,
+    tactic.trace "refine CreateAll",
     scs ← zipper.lowest_uncommon_subterms ce $ zipper.zip a,
     if scs.length = 0 then notimpl else do
     let scs := task.Create <$> zipper.current <$> scs,
@@ -160,7 +199,7 @@ end
 
 meta def strategy.execute : strategy → conv unit
 |(strategy.ReduceDistance a b) := notimpl
-|(strategy.Use r)              := rule.to_conv r
+|s@(strategy.Use r)              := zipper.rewrite_conv r
 open tactic
 meta def strategy.refine : strategy → M refinement
 |(strategy.ReduceDistance a b) := notimpl
@@ -189,11 +228,15 @@ meta def explore_tasks : list (task × stack) → list (strategy × stack) → M
 |[] acc := pure acc
 |((t,st) :: rest) acc := do
     state ← get,
-    is_achieved ← task.test t,
+    ce ← get_ce,
+    is_achieved ← task.test ce t,
+    tactic.trace_m "explore_tasks: " $ t,
     if is_achieved then explore_tasks rest acc else do
     (subtasks, substrats) ← task.refine t,
-    let subtasks := st.append_subtasks $ subtasks.filter (λ t, stack.has_task st t), -- filter out subtasks that are already on the stack.
-    let substrats := st.append_substrats $ substrats.filter (λ s, stack.has_strat st s),
+    pp_st ← pp subtasks, pp_ss ← pp substrats,
+    trace_m "explore_tasks: " $ (to_fmt "found: " ++ pp_st ++ ", " ++ pp_ss),
+    let subtasks := st.append_subtasks $ subtasks.filter (λ t, ¬ stack.has_task st t), -- filter out subtasks that are already on the stack.
+    let substrats := st.append_substrats $ substrats.filter (λ s, ¬ stack.has_strat st s),
     let acc := substrats ++ acc,
     explore_tasks (subtasks ++ rest) acc
 
@@ -205,18 +248,26 @@ meta def explore_strategy : (strategy × stack) → M (list (strategy × stack))
     (subtasks, substrats) ← strategy.refine s,
     explore_tasks (stack.append_subtasks subtasks) (stack.append_substrats substrats)
 
+meta def explore : stack → M (list (strategy × stack))
+|[] := failure
+|s@((stack_entry.task t _ _) :: _) := explore_task (t,s)
+|s@((stack_entry.strategy t) :: _) := explore_strategy (t,s)
+
 meta def execute_strategy : strategy → stack → M unit
-|s stack := do
+|s rest := do
     state ← get,
     ce ← get_ce,
+    trace_m "execute_strategy: " $ s,
     state_t.lift $ strategy.execute s,
     ce' ← get_ce,
     when (ce = ce') (tactic.fail "strategy did not change the goal."),
+    trace_m "execute_strategy: " $ (list.tail rest),
     stack.mfold_achieved (λ _ acheived, do 
-        r ← acheived.test, 
-        when (r) (tactic.fail "stategy caused a previously achieved task to fail.")
-    ) (),
-    lookahead ← rule_table.rewrites ce' state.config.rule_table,
+        r ← acheived.test ce', 
+        when (¬r) (tactic.fail "stategy caused a previously achieved task to fail.")
+    ) () $ list.tail $ rest,
+    trace "hi",
+    lookahead ← rule_table.rewrites ce' state.rt,
     let visited := state.visited.insert ce,
     put {
         state with
@@ -225,12 +276,15 @@ meta def execute_strategy : strategy → stack → M unit
     }
 
 meta def ascend : stack → M (list (strategy × stack))
-|[] := pure []
-|stack@((stack_entry.strategy s)::t) :=
-    (execute_strategy s stack *> ascend t) 
-    <|> (explore_strategy (s,stack))
+|[] := do trace_m "ascend: " $ "done!", pure []
+|stack@((stack_entry.strategy s)::t) := do
+    trace_m "ascend: " $ s,
+    (do execute_strategy s stack, ascend t) 
+    <|> (do trace "ascend: execute_strategy failed", explore_strategy (s,stack))
 |stack@((stack_entry.task current siblings achieved) :: tail) := do
-    is_achieved ← task.test current,
+    trace_m "ascend: " $ current,
+    ce ← get_ce,
+    is_achieved ← task.test ce current,
     if (is_achieved) then
         let achieved := current::achieved in
         match siblings with
@@ -245,6 +299,46 @@ meta def ascend : stack → M (list (strategy × stack))
 meta def execute : (strategy × stack) → M (list (strategy × stack))
 | ⟨strat, t⟩ := ascend t
 
+meta def init (rt : rule_table) : M (list (strategy × stack)) := do
+    (_,lhs,rhs) ← target_lhs_rhs,
+    lookahead ← rt.rewrites lhs,
+    put $ {
+        lookahead := lookahead,
+        visited := ∅,
+        rt := rt
+    },
+    t ← pure $ task.CreateAll rhs,
+    explore_task (t, [stack_entry.task t [] []])
+
+meta def policy := list (strategy × stack) → M (strategy × stack)
+
+/--A simple policy that just tries the first one. -/
+meta def first_policy : policy
+|[] := failure
+|l@(h::t) := do
+    pph ← pp h.1,
+    ppl ← pp $ list.map prod.fst l,
+    trace_m "first_policy: " $ (to_fmt "choose ") ++ ppl,
+    pure h
+
+meta def run_aux (π : policy) : state → list (strategy × stack) → nat → conv unit
+|s [] n := pure ()
+|_ _ 0 := fail "timeout"
+|s l (n+1) := do
+    target >>= trace_m "run_aux: ",
+
+    ⟨r,s⟩ ← state_t.run (π l >>= execute) $ s,
+    run_aux s r n
+
+meta def run (π : policy) (rt : rule_table) : conv unit := do
+    trace "robot.run: ()",
+    (_,lhs, rhs) ← target_lhs_rhs,
+    lookahead ← rt.rewrites lhs,
+    let s : state := {lookahead := lookahead, visited := ∅, rt := rt},
+    let t := task.CreateAll rhs,
+    ⟨r,s⟩ ←  state_t.run (explore_task (t, [stack_entry.task t [] []])) s,
+    -- trace r,
+    run_aux π s r 10
 
 
 end robot
